Undo accidental changes.

thys/Abstract_Completeness/Abstract_Completeness.thy
@@ -12,79 +12,78 @@ begin
 
 section\<open>General Tree Concepts\<close>
 
-codatatype 'a tree = Node (root: 'a) (cont: \<open>'a tree fset\<close>)
+codatatype 'a tree = Node (root: 'a) (cont: "'a tree fset")
 
 inductive tfinite where
-  tfinite: \<open>(\<And> t'. t' |\<in>| cont t \<Longrightarrow> tfinite t') \<Longrightarrow> tfinite t\<close>
+  tfinite: "(\<And> t'. t' |\<in>| cont t \<Longrightarrow> tfinite t') \<Longrightarrow> tfinite t"
 
 
 (*<*)(* Infinite paths in trees. *)(*>*)
 coinductive ipath where
-  ipath: \<open>\<lbrakk>root t = shd steps; t' |\<in>| cont t; ipath t' (stl steps)\<rbrakk> \<Longrightarrow> ipath t steps\<close>
+  ipath: "\<lbrakk>root t = shd steps; t' |\<in>| cont t; ipath t' (stl steps)\<rbrakk> \<Longrightarrow> ipath t steps"
 
 (*<*)(* Finite trees have no infinite paths. *)
-lemma ftree_no_ipath: \<open>tfinite t \<Longrightarrow> \<not> ipath t steps\<close>
+lemma ftree_no_ipath: "tfinite t \<Longrightarrow> \<not> ipath t steps"
   by (induct t arbitrary: steps rule: tfinite.induct) (auto elim: ipath.cases)
 (*>*)
 
 primcorec konig where
-  \<open>shd (konig t) = root t\<close>
-| \<open>stl (konig t) = konig (SOME t'. t' |\<in>| cont t \<and> \<not> tfinite t')\<close>
+  "shd (konig t) = root t"
+| "stl (konig t) = konig (SOME t'. t' |\<in>| cont t \<and> \<not> tfinite t')"
 
-lemma Konig: \<open>\<not> tfinite t \<Longrightarrow> ipath t (konig t)\<close>
+lemma Konig: "\<not> tfinite t \<Longrightarrow> ipath t (konig t)"
   by (coinduction arbitrary: t) (metis (lifting) tfinite.simps konig.simps someI_ex)
 
 
 section\<open>Rule Systems\<close>
 
 (*<*)(* A step consists of a pair (s,r) such that the rule r is taken in state s. *)(*>*)
-type_synonym ('state, 'rule) step = \<open>'state \<times> 'rule\<close>
-
+type_synonym ('state, 'rule) step = "'state \<times> 'rule"
 (*<*)(* A derivation tree is a tree of steps: *)(*>*)
-type_synonym ('state, 'rule) dtree = \<open>('state, 'rule) step tree\<close>
+type_synonym ('state, 'rule) dtree = "('state, 'rule) step tree"
 
 locale RuleSystem_Defs =
-fixes eff :: \<open>'rule \<Rightarrow> 'state \<Rightarrow> 'state fset \<Rightarrow> bool\<close>
+fixes eff :: "'rule \<Rightarrow> 'state \<Rightarrow> 'state fset \<Rightarrow> bool"
 (* The countable set of rules is initially provided as a stream: *)
-and rules :: \<open>'rule stream\<close>
+and rules :: "'rule stream"
 begin
 
-abbreviation \<open>R \<equiv> sset rules\<close>
+abbreviation "R \<equiv> sset rules"
 
-lemma countable_R: \<open>countable R\<close> by (metis countableI_type countable_image sset_range)
-lemma NE_R: \<open>R \<noteq> {}\<close> by (metis UNIV_witness all_not_in_conv empty_is_image sset_range)
+lemma countable_R: "countable R" by (metis countableI_type countable_image sset_range)
+lemma NE_R: "R \<noteq> {}" by (metis UNIV_witness all_not_in_conv empty_is_image sset_range)
 
-definition \<open>enabled r s \<equiv> \<exists> sl. eff r s sl\<close>
-definition \<open>pickEff r s \<equiv> if enabled r s then (SOME sl. eff r s sl) else the None\<close>
+definition "enabled r s \<equiv> \<exists> sl. eff r s sl"
+definition "pickEff r s \<equiv> if enabled r s then (SOME sl. eff r s sl) else the None"
 
-lemma pickEff: \<open>enabled r s \<Longrightarrow> eff r s (pickEff r s)\<close>
+lemma pickEff: "enabled r s \<Longrightarrow> eff r s (pickEff r s)"
   by (metis enabled_def pickEff_def tfl_some)
 
-abbreviation \<open>effStep step \<equiv> eff (snd step) (fst step)\<close>
-abbreviation \<open>enabledAtStep r step \<equiv> enabled r (fst step)\<close>
-abbreviation \<open>takenAtStep r step \<equiv> snd step = r\<close>
+abbreviation "effStep step \<equiv> eff (snd step) (fst step)"
+abbreviation "enabledAtStep r step \<equiv> enabled r (fst step)"
+abbreviation "takenAtStep r step \<equiv> snd step = r"
 
 text \<open>Saturation is a very strong notion of fairness:
   If a rule is enabled at some point, it will eventually be taken.\<close>
-definition \<open>saturated r \<equiv> alw (holds (enabledAtStep r) impl ev (holds (takenAtStep r)))\<close>
-definition \<open>Saturated steps \<equiv> \<forall> r \<in> R. saturated r steps\<close>
+definition "saturated r \<equiv> alw (holds (enabledAtStep r) impl ev (holds (takenAtStep r)))"
+definition "Saturated steps \<equiv> \<forall> r \<in> R. saturated r steps"
 
 (*<*)(* Well-formed derivation trees *)(*>*)
 coinductive wf where
-  wf: \<open>\<lbrakk>snd (root t) \<in> R; effStep (root t) (fimage (fst o root) (cont t));
-    \<And>t'. t' |\<in>| cont t \<Longrightarrow> wf t'\<rbrakk> \<Longrightarrow> wf t\<close>
+  wf: "\<lbrakk>snd (root t) \<in> R; effStep (root t) (fimage (fst o root) (cont t));
+    \<And>t'. t' |\<in>| cont t \<Longrightarrow> wf t'\<rbrakk> \<Longrightarrow> wf t"
 
 
 (*<*)(* Escape paths *)(*>*)
 coinductive epath where
-  epath: \<open>\<lbrakk>snd (shd steps) \<in> R; fst (shd (stl steps)) |\<in>| sl; effStep (shd steps) sl;
-    epath (stl steps)\<rbrakk> \<Longrightarrow> epath steps\<close>
+  epath: "\<lbrakk>snd (shd steps) \<in> R; fst (shd (stl steps)) |\<in>| sl; effStep (shd steps) sl;
+    epath (stl steps)\<rbrakk> \<Longrightarrow> epath steps"
 
 lemma wf_ipath_epath:
-  assumes \<open>wf t\<close> \<open>ipath t steps\<close>
-  shows \<open>epath steps\<close>
+  assumes "wf t" "ipath t steps"
+  shows "epath steps"
 proof -
-  have *: \<open>\<And>t st. ipath t st \<Longrightarrow> root t = shd st\<close> by (auto elim: ipath.cases)
+  have *: "\<And>t st. ipath t st \<Longrightarrow> root t = shd st" by (auto elim: ipath.cases)
   show ?thesis using assms
   proof (coinduction arbitrary: t steps)
     case epath
@@ -92,231 +91,231 @@ proof -
   qed
 qed
 
-definition \<open>fair rs \<equiv> sset rs \<subseteq> R \<and> (\<forall> r \<in> R. alw (ev (holds ((=) r))) rs)\<close>
+definition "fair rs \<equiv> sset rs \<subseteq> R \<and> (\<forall> r \<in> R. alw (ev (holds ((=) r))) rs)"
 
-lemma fair_stl: \<open>fair rs \<Longrightarrow> fair (stl rs)\<close>
+lemma fair_stl: "fair rs \<Longrightarrow> fair (stl rs)"
   unfolding fair_def by (metis alw.simps subsetD stl_sset subsetI)
 
-lemma sdrop_fair: \<open>fair rs \<Longrightarrow> fair (sdrop m rs)\<close>
+lemma sdrop_fair: "fair rs \<Longrightarrow> fair (sdrop m rs)"
   using alw_sdrop unfolding fair_def by (metis alw.coinduct alw_nxt fair_def fair_stl)
 
 
 section\<open>A Fair Enumeration of the Rules\<close>
 
 (*<*)(* The fair enumeration of rules *)(*>*)
-definition \<open>fenum \<equiv> flat (smap (\<lambda>n. stake n rules) (fromN 1))\<close>
+definition "fenum \<equiv> flat (smap (\<lambda>n. stake n rules) (fromN 1))"
 
-lemma sset_fenum: \<open>sset fenum = R\<close>
+lemma sset_fenum: "sset fenum = R"
   unfolding fenum_def by (subst sset_flat)
    (auto simp: stream.set_map in_set_conv_nth sset_range[of rules],
      metis atLeast_Suc_greaterThan greaterThan_0 lessI range_eqI stake_nth)
 
-lemma fair_fenum: \<open>fair fenum\<close>
+lemma fair_fenum: "fair fenum"
 proof -
-  { fix r assume \<open>r \<in> R\<close>
-    then obtain m where r: \<open>r = rules !! m\<close> unfolding sset_range by blast
-    { fix n :: nat and rs let ?fenum = \<open>\<lambda>n. flat (smap (\<lambda>n. stake n rules) (fromN n))\<close>
-      assume \<open>n > 0\<close>
-      hence \<open>alw (ev (holds ((=) r))) (rs @- ?fenum n)\<close>
+  { fix r assume "r \<in> R"
+    then obtain m where r: "r = rules !! m" unfolding sset_range by blast
+    { fix n :: nat and rs let ?fenum = "\<lambda>n. flat (smap (\<lambda>n. stake n rules) (fromN n))"
+      assume "n > 0"
+      hence "alw (ev (holds ((=) r))) (rs @- ?fenum n)"
       proof (coinduction arbitrary: n rs)
         case alw
         show ?case
-        proof (rule exI[of _ \<open>rs @- ?fenum n\<close>], safe)
-          show \<open>\<exists>n' rs'. stl (rs @- ?fenum n) = rs' @- ?fenum n' \<and> n' > 0\<close>
+        proof (rule exI[of _ "rs @- ?fenum n"], safe)
+          show "\<exists>n' rs'. stl (rs @- ?fenum n) = rs' @- ?fenum n' \<and> n' > 0"
           proof(cases rs)
             case Nil thus ?thesis unfolding alw by (intro exI) auto
           qed (auto simp: alw intro: exI[of _ n])
         next
-          show \<open>ev (holds ((=) r)) (rs @- flat (smap (\<lambda>n. stake n rules) (fromN n)))\<close>
+          show "ev (holds ((=) r)) (rs @- flat (smap (\<lambda>n. stake n rules) (fromN n)))"
             using alw r unfolding ev_holds_sset
-            by (cases \<open>m < n\<close>) (force simp: stream.set_map in_set_conv_nth)+
+            by (cases "m < n") (force simp: stream.set_map in_set_conv_nth)+
         qed
      qed
     }
   }
-  thus \<open>fair fenum\<close> unfolding fair_def sset_fenum
+  thus "fair fenum" unfolding fair_def sset_fenum
     by (metis fenum_def alw_shift le_less zero_less_one)
 qed
 
-definition \<open>trim rs s = sdrop_while (\<lambda>r. Not (enabled r s)) rs\<close>
+definition "trim rs s = sdrop_while (\<lambda>r. Not (enabled r s)) rs"
 
 
 (*<*)(* The fair tree associated to a stream of rules and a state *)(*>*)
 primcorec mkTree where
-  \<open>root (mkTree rs s) = (s, (shd (trim rs s)))\<close>
-| \<open>cont (mkTree rs s) = fimage (mkTree (stl (trim rs s))) (pickEff (shd (trim rs s)) s)\<close>
+  "root (mkTree rs s) = (s, (shd (trim rs s)))"
+| "cont (mkTree rs s) = fimage (mkTree (stl (trim rs s))) (pickEff (shd (trim rs s)) s)"
 
 (*<*)(* More efficient code equation for mkTree *)(*>*)
-lemma mkTree_unfold[code]:
-  \<open>mkTree rs s = (case trim rs s of SCons r s' \<Rightarrow> Node (s, r) (fimage (mkTree s') (pickEff r s)))\<close>
+lemma mkTree_unfold[code]: "mkTree rs s =
+  (case trim rs s of SCons r s' \<Rightarrow> Node (s, r) (fimage (mkTree s') (pickEff r s)))"
   by (subst mkTree.ctr) (simp split: stream.splits)
 
 end
 
 locale RuleSystem = RuleSystem_Defs eff rules
-for eff :: \<open>'rule \<Rightarrow> 'state \<Rightarrow> 'state fset \<Rightarrow> bool\<close> and rules :: \<open>'rule stream\<close> +
-fixes S :: \<open>'state set\<close>
-assumes eff_S: \<open>\<And> s r sl s'. \<lbrakk>s \<in> S; r \<in> R; eff r s sl; s' |\<in>| sl\<rbrakk> \<Longrightarrow> s' \<in> S\<close>
-and enabled_R: \<open>\<And> s. s \<in> S \<Longrightarrow> \<exists> r \<in> R. \<exists> sl. eff r s sl\<close>
+for eff :: "'rule \<Rightarrow> 'state \<Rightarrow> 'state fset \<Rightarrow> bool" and rules :: "'rule stream" +
+fixes S :: "'state set"
+assumes eff_S: "\<And> s r sl s'. \<lbrakk>s \<in> S; r \<in> R; eff r s sl; s' |\<in>| sl\<rbrakk> \<Longrightarrow> s' \<in> S"
+and enabled_R: "\<And> s. s \<in> S \<Longrightarrow> \<exists> r \<in> R. \<exists> sl. eff r s sl"
 begin
 
 (*<*)(* The minimum waiting time in a stream for the enabled rules in a given state: *)(*>*)
-definition \<open>minWait rs s \<equiv> LEAST n. enabled (shd (sdrop n rs)) s\<close>
+definition "minWait rs s \<equiv> LEAST n. enabled (shd (sdrop n rs)) s"
 
 lemma trim_alt:
-  assumes s: \<open>s \<in> S\<close> and rs: \<open>fair rs\<close>
-  shows \<open>trim rs s = sdrop (minWait rs s) rs\<close>
+  assumes s: "s \<in> S" and rs: "fair rs"
+  shows "trim rs s = sdrop (minWait rs s) rs"
 proof (unfold trim_def minWait_def sdrop_simps, rule sdrop_while_sdrop_LEAST[unfolded o_def])
-  from enabled_R[OF s] obtain r sl where r: \<open>r \<in> R\<close> and sl: \<open>eff r s sl\<close> by blast
-  from bspec[OF conjunct2[OF rs[unfolded fair_def]] r] obtain m where \<open>r = rs !! m\<close>
+  from enabled_R[OF s] obtain r sl where r: "r \<in> R" and sl: "eff r s sl" by blast
+  from bspec[OF conjunct2[OF rs[unfolded fair_def]] r] obtain m where "r = rs !! m"
     by atomize_elim (erule alw.cases, auto simp only: ev_holds_sset sset_range)
-  with r sl show \<open>\<exists>n. enabled (rs !! n) s\<close> unfolding enabled_def by auto
+  with r sl show "\<exists>n. enabled (rs !! n) s" unfolding enabled_def by auto
 qed
 
 lemma minWait_ex:
-  assumes s: \<open>s \<in> S\<close> and rs: \<open>fair rs\<close>
-  shows \<open>\<exists> n. enabled (shd (sdrop n rs)) s\<close>
+  assumes s: "s \<in> S" and rs: "fair rs"
+  shows "\<exists> n. enabled (shd (sdrop n rs)) s"
 proof -
-  obtain r where r: \<open>r \<in> R\<close> and e: \<open>enabled r s\<close> using enabled_R s unfolding enabled_def by blast
-  then obtain n where \<open>shd (sdrop n rs) = r\<close> using sdrop_fair[OF rs]
+  obtain r where r: "r \<in> R" and e: "enabled r s" using enabled_R s unfolding enabled_def by blast
+  then obtain n where "shd (sdrop n rs) = r" using sdrop_fair[OF rs]
     by (metis (full_types) alw_nxt holds.simps sdrop.simps(1) fair_def sdrop_wait)
   thus ?thesis using r e by auto
 qed
 
-lemma assumes \<open>s \<in> S\<close> and \<open>fair rs\<close>
-  shows trim_in_R: \<open>shd (trim rs s) \<in> R\<close>
-  and trim_enabled: \<open>enabled (shd (trim rs s)) s\<close>
-  and trim_fair: \<open>fair (trim rs s)\<close>
+lemma assumes "s \<in> S" and "fair rs"
+  shows trim_in_R: "shd (trim rs s) \<in> R"
+  and trim_enabled: "enabled (shd (trim rs s)) s"
+  and trim_fair: "fair (trim rs s)"
   unfolding trim_alt[OF assms] minWait_def
   using LeastI_ex[OF minWait_ex[OF assms]] sdrop_fair[OF assms(2)]
     conjunct1[OF assms(2)[unfolded fair_def]] by simp_all (metis subsetD snth_sset)
 
-lemma minWait_least: \<open>\<lbrakk>enabled (shd (sdrop n rs)) s\<rbrakk> \<Longrightarrow> minWait rs s \<le> n\<close>
+lemma minWait_least: "\<lbrakk>enabled (shd (sdrop n rs)) s\<rbrakk> \<Longrightarrow> minWait rs s \<le> n"
   unfolding minWait_def by (intro Least_le conjI)
 
 lemma in_cont_mkTree:
-  assumes s: \<open>s \<in> S\<close> and rs: \<open>fair rs\<close> and t': \<open>t' |\<in>| cont (mkTree rs s)\<close>
-  shows \<open>\<exists> sl' s'. s' \<in> S \<and> eff (shd (trim rs s)) s sl' \<and>
-                 s' |\<in>| sl' \<and> t' = mkTree (stl (trim rs s)) s'\<close>
+  assumes s: "s \<in> S" and rs: "fair rs" and t': "t' |\<in>| cont (mkTree rs s)"
+  shows "\<exists> sl' s'. s' \<in> S \<and> eff (shd (trim rs s)) s sl' \<and>
+                 s' |\<in>| sl' \<and> t' = mkTree (stl (trim rs s)) s'"
 proof -
-  define sl' where \<open>sl' = pickEff (shd (trim rs s)) s\<close>
-  obtain s' where s': \<open>s' |\<in>| sl'\<close> and \<open>t' = mkTree (stl (trim rs s)) s'\<close>
+  define sl' where "sl' = pickEff (shd (trim rs s)) s"
+  obtain s' where s': "s' |\<in>| sl'" and "t' = mkTree (stl (trim rs s)) s'"
     using t' unfolding sl'_def by auto
-  moreover have 1: \<open>enabled (shd (trim rs s)) s\<close> using trim_enabled[OF s rs] .
-  moreover with trim_in_R pickEff eff_S s rs s'[unfolded sl'_def] have \<open>s' \<in> S\<close> by blast
+  moreover have 1: "enabled (shd (trim rs s)) s" using trim_enabled[OF s rs] .
+  moreover with trim_in_R pickEff eff_S s rs s'[unfolded sl'_def] have "s' \<in> S" by blast
   ultimately show ?thesis unfolding sl'_def using pickEff by blast
 qed
 
 lemma ipath_mkTree_sdrop:
-  assumes s: \<open>s \<in> S\<close> and rs: \<open>fair rs\<close> and i: \<open>ipath (mkTree rs s) steps\<close>
-  shows \<open>\<exists> n s'. s' \<in> S \<and> ipath (mkTree (sdrop n rs) s') (sdrop m steps)\<close>
+  assumes s: "s \<in> S" and rs: "fair rs" and i: "ipath (mkTree rs s) steps"
+  shows "\<exists> n s'. s' \<in> S \<and> ipath (mkTree (sdrop n rs) s') (sdrop m steps)"
 using s rs i proof (induct m arbitrary: steps rs)
   case (Suc m)
-  then obtain n s' where s': \<open>s' \<in> S\<close>
-    and ip: \<open>ipath (mkTree (sdrop n rs) s') (sdrop m steps)\<close> (is \<open>ipath ?t _\<close>) by blast
-  from ip obtain t' where r: \<open>root ?t = shd (sdrop m steps)\<close> and t': \<open>t' |\<in>| cont ?t\<close>
-    and i: \<open>ipath t' (sdrop (Suc m) steps)\<close> by (cases, simp)
+  then obtain n s' where s': "s' \<in> S"
+    and ip: "ipath (mkTree (sdrop n rs) s') (sdrop m steps)" (is "ipath ?t _") by blast
+  from ip obtain t' where r: "root ?t = shd (sdrop m steps)" and t': "t' |\<in>| cont ?t"
+    and i: "ipath t' (sdrop (Suc m) steps)" by (cases, simp)
   from in_cont_mkTree[OF s' sdrop_fair[OF Suc.prems(2)] t'] obtain sl'' s'' where
-    e: \<open>eff (shd (trim (sdrop n rs) s')) s' sl''\<close> and
-    s'': \<open>s'' |\<in>| sl''\<close> and t'_def: \<open>t' = mkTree (stl (trim (sdrop n rs) s')) s''\<close> by blast
-  have \<open>shd (trim (sdrop n rs) s') \<in> R\<close> by (metis sdrop_fair Suc.prems(2) trim_in_R s')
+    e: "eff (shd (trim (sdrop n rs) s')) s' sl''" and
+    s'': "s'' |\<in>| sl''" and t'_def: "t' = mkTree (stl (trim (sdrop n rs) s')) s''" by blast
+  have "shd (trim (sdrop n rs) s') \<in> R" by (metis sdrop_fair Suc.prems(2) trim_in_R s')
   thus ?case using i s'' e s' unfolding sdrop_stl t'_def sdrop_add add.commute[of n]
     trim_alt[OF s' sdrop_fair[OF Suc.prems(2)]]
-    by (intro exI[of _ \<open>minWait (sdrop n rs) s' + Suc n\<close>] exI[of _ s'']) (simp add: eff_S)
+    by (intro exI[of _ "minWait (sdrop n rs) s' + Suc n"] exI[of _ s'']) (simp add: eff_S)
 qed (auto intro!: exI[of _ 0] exI[of _ s])
 
 lemma wf_mkTree:
-  assumes s: \<open>s \<in> S\<close> and \<open>fair rs\<close>
-  shows \<open>wf (mkTree rs s)\<close>
+  assumes s: "s \<in> S" and "fair rs"
+  shows "wf (mkTree rs s)"
 using assms proof (coinduction arbitrary: rs s)
-  case (wf rs s) let ?t = \<open>mkTree rs s\<close>
-  have \<open>snd (root ?t) \<in> R\<close> using trim_in_R[OF wf] by simp
-  moreover have \<open>fst \<circ> root \<circ> mkTree (stl (trim rs s)) = id\<close> by auto
-  hence \<open>effStep (root ?t) (fimage (fst \<circ> root) (cont ?t))\<close>
+  case (wf rs s) let ?t = "mkTree rs s"
+  have "snd (root ?t) \<in> R" using trim_in_R[OF wf] by simp
+  moreover have "fst \<circ> root \<circ> mkTree (stl (trim rs s)) = id" by auto
+  hence "effStep (root ?t) (fimage (fst \<circ> root) (cont ?t))"
     using trim_enabled[OF wf] by (simp add: pickEff)
   ultimately show ?case using fair_stl[OF trim_fair[OF wf]] in_cont_mkTree[OF wf]
-    by (auto intro!: exI[of _ \<open>stl (trim rs s)\<close>])
+    by (auto intro!: exI[of _ "stl (trim rs s)"])
 qed
 
 
 (*<*)(* The position of a rule in a rule stream *)(*>*)
-definition \<open>pos rs r \<equiv> LEAST n. shd (sdrop n rs) = r\<close>
+definition "pos rs r \<equiv> LEAST n. shd (sdrop n rs) = r"
 
-lemma pos: \<open>\<lbrakk>fair rs; r \<in> R\<rbrakk> \<Longrightarrow> shd (sdrop (pos rs r) rs) = r\<close>
+lemma pos: "\<lbrakk>fair rs; r \<in> R\<rbrakk> \<Longrightarrow> shd (sdrop (pos rs r) rs) = r"
   unfolding pos_def
   by (rule LeastI_ex) (metis (full_types) alw.cases fair_def holds.simps sdrop_wait)
 
-lemma pos_least: \<open>shd (sdrop n rs) = r \<Longrightarrow> pos rs r \<le> n\<close>
+lemma pos_least: "shd (sdrop n rs) = r \<Longrightarrow> pos rs r \<le> n"
   unfolding pos_def by (metis (full_types) Least_le)
 
-lemma minWait_le_pos: \<open>\<lbrakk>fair rs; r \<in> R; enabled r s\<rbrakk> \<Longrightarrow> minWait rs s \<le> pos rs r\<close>
+lemma minWait_le_pos: "\<lbrakk>fair rs; r \<in> R; enabled r s\<rbrakk> \<Longrightarrow> minWait rs s \<le> pos rs r"
   by (auto simp del: sdrop_simps intro: minWait_least simp: pos)
 
 lemma stake_pos_minWait:
-  assumes rs: \<open>fair rs\<close> and m: \<open>minWait rs s < pos rs r\<close> and r: \<open>r \<in> R\<close> and s: \<open>s \<in> S\<close>
-  shows \<open>pos (stl (trim rs s)) r = pos rs r - Suc (minWait rs s)\<close>
+  assumes rs: "fair rs" and m: "minWait rs s < pos rs r" and r: "r \<in> R" and s: "s \<in> S"
+  shows "pos (stl (trim rs s)) r = pos rs r - Suc (minWait rs s)"
 proof -
-  have \<open>pos rs r - Suc (minWait rs s) + minWait rs s = pos rs r - Suc 0\<close> using m by auto
-  moreover have \<open>shd (stl (sdrop (pos rs r - Suc 0) rs)) = shd (sdrop (pos rs r) rs)\<close>
+  have "pos rs r - Suc (minWait rs s) + minWait rs s = pos rs r - Suc 0" using m by auto
+  moreover have "shd (stl (sdrop (pos rs r - Suc 0) rs)) = shd (sdrop (pos rs r) rs)"
     by (metis Suc_pred gr_implies_not0 m neq0_conv sdrop.simps(2) sdrop_stl)
-  ultimately have \<open>pos (stl (trim rs s)) r \<le> pos rs r - Suc (minWait rs s)\<close>
+  ultimately have "pos (stl (trim rs s)) r \<le> pos rs r - Suc (minWait rs s)"
     using pos[OF rs r] by (auto simp: add.commute trim_alt[OF s rs] intro: pos_least)
   moreover
-  have \<open>pos rs r \<le> pos (stl (trim rs s)) r + Suc (minWait rs s)\<close>
-    using pos[OF sdrop_fair[OF fair_stl[OF rs]] r, of \<open>minWait rs s\<close>]
+  have "pos rs r \<le> pos (stl (trim rs s)) r + Suc (minWait rs s)"
+    using pos[OF sdrop_fair[OF fair_stl[OF rs]] r, of "minWait rs s"]
     by (auto simp: trim_alt[OF s rs] add.commute intro: pos_least)
-  hence \<open>pos rs r - Suc (minWait rs s) \<le> pos (stl (trim rs s)) r\<close> by linarith
+  hence "pos rs r - Suc (minWait rs s) \<le> pos (stl (trim rs s)) r" by linarith
   ultimately show ?thesis by simp
 qed
 
 lemma ipath_mkTree_ev:
-  assumes s: \<open>s \<in> S\<close> and rs: \<open>fair rs\<close>
-  and i: \<open>ipath (mkTree rs s) steps\<close> and r: \<open>r \<in> R\<close>
-  and alw: \<open>alw (holds (enabledAtStep r)) steps\<close>
-  shows \<open>ev (holds (takenAtStep r)) steps\<close>
-using s rs i alw proof (induction \<open>pos rs r\<close> arbitrary: rs s steps rule: less_induct)
+  assumes s: "s \<in> S" and rs: "fair rs"
+  and i: "ipath (mkTree rs s) steps" and r: "r \<in> R"
+  and alw: "alw (holds (enabledAtStep r)) steps"
+  shows "ev (holds (takenAtStep r)) steps"
+using s rs i alw proof (induction "pos rs r" arbitrary: rs s steps rule: less_induct)
   case (less rs s steps) note s = \<open>s \<in> S\<close> and trim_def' = trim_alt[OF s \<open>fair rs\<close>]
-  let ?t = \<open>mkTree rs s\<close>
-  from less(4,3) s in_cont_mkTree obtain t' :: \<open>('state, 'rule) step tree\<close> and s' where
-    rt: \<open>root ?t = shd steps\<close> and i: \<open>ipath (mkTree (stl (trim rs s)) s') (stl steps)\<close> and
-    s': \<open>s' \<in> S\<close> by cases fast
+  let ?t = "mkTree rs s"
+  from less(4,3) s in_cont_mkTree obtain t' :: "('state, 'rule) step tree" and s' where
+    rt: "root ?t = shd steps" and i: "ipath (mkTree (stl (trim rs s)) s') (stl steps)" and
+    s': "s' \<in> S" by cases fast
   show ?case
-  proof(cases \<open>pos rs r = minWait rs s\<close>)
+  proof(cases "pos rs r = minWait rs s")
     case True
     with pos[OF less.prems(2) r] rt[symmetric] show ?thesis by (auto simp: trim_def' ev.base)
   next
     case False
-    have e: \<open>enabled r s\<close> using less.prems(4) rt  by (subst (asm) alw_nxt, cases steps) auto
-    with False r less.prems(2) have 2: \<open>minWait rs s < pos rs r\<close> using minWait_le_pos by force
-    let ?m1 = \<open>pos rs r - Suc (minWait rs s)\<close>
-    have \<open>Suc ?m1 \<le> pos rs r\<close> using 2 by auto
-    moreover have \<open>?m1 = pos (stl (trim rs s)) r\<close> using e \<open>fair rs\<close> 2 r s
+    have e: "enabled r s" using less.prems(4) rt  by (subst (asm) alw_nxt, cases steps) auto
+    with False r less.prems(2) have 2: "minWait rs s < pos rs r" using minWait_le_pos by force
+    let ?m1 = "pos rs r - Suc (minWait rs s)"
+    have "Suc ?m1 \<le> pos rs r" using 2 by auto
+    moreover have "?m1 = pos (stl (trim rs s)) r" using e \<open>fair rs\<close> 2 r s
       by (auto intro: stake_pos_minWait[symmetric])
-    moreover have \<open>fair (stl (trim rs s))\<close> \<open>alw (holds (enabledAtStep r)) (stl steps)\<close>
+    moreover have "fair (stl (trim rs s))" "alw (holds (enabledAtStep r)) (stl steps)"
       using less.prems by (metis fair_stl trim_fair, metis alw.simps)
-    ultimately show \<open>?thesis\<close> by (auto intro: ev.step[OF less.hyps[OF _ s' _ i]])
+    ultimately show "?thesis" by (auto intro: ev.step[OF less.hyps[OF _ s' _ i]])
   qed
 qed
 
 section\<open>Persistent rules\<close>
 
 definition
-  \<open>per r \<equiv>
-    \<forall>s r1 sl' s'. s \<in> S \<and> enabled r s \<and> r1 \<in> R - {r} \<and> eff r1 s sl' \<and> s' |\<in>| sl' \<longrightarrow> enabled r s'\<close>
+  "per r \<equiv>
+    \<forall>s r1 sl' s'. s \<in> S \<and> enabled r s \<and> r1 \<in> R - {r} \<and> eff r1 s sl' \<and> s' |\<in>| sl' \<longrightarrow> enabled r s'"
 
 lemma per_alw:
-  assumes p: \<open>per r\<close> and e: \<open>epath steps \<and> fst (shd steps) \<in> S\<close>
-  shows \<open>alw (holds (enabledAtStep r) impl
-    (holds (takenAtStep r) or nxt (holds (enabledAtStep r)))) steps\<close>
+  assumes p: "per r" and e: "epath steps \<and> fst (shd steps) \<in> S"
+  shows "alw (holds (enabledAtStep r) impl
+    (holds (takenAtStep r) or nxt (holds (enabledAtStep r)))) steps"
 using e proof coinduct
   case (alw steps)
   moreover
-  { let ?s = \<open>fst (shd steps)\<close>  let ?r1 = \<open>snd (shd steps)\<close>
-    let ?s' = \<open>fst (shd (stl steps))\<close>
-    assume \<open>?s \<in> S\<close> and \<open>enabled r ?s\<close> and \<open>?r1 \<noteq> r\<close>
-    moreover have \<open>?r1 \<in> R\<close> using alw by (auto elim: epath.cases)
-    moreover obtain sl' where \<open>eff ?r1 ?s sl' \<and> ?s' |\<in>| sl'\<close> using alw by (auto elim: epath.cases)
-    ultimately have \<open>enabled r ?s'\<close> using p unfolding per_def by blast
+  { let ?s = "fst (shd steps)"  let ?r1 = "snd (shd steps)"
+    let ?s' = "fst (shd (stl steps))"
+    assume "?s \<in> S" and "enabled r ?s" and "?r1 \<noteq> r"
+    moreover have "?r1 \<in> R" using alw by (auto elim: epath.cases)
+    moreover obtain sl' where "eff ?r1 ?s sl' \<and> ?s' |\<in>| sl'" using alw by (auto elim: epath.cases)
+    ultimately have "enabled r ?s'" using p unfolding per_def by blast
   }
   ultimately show ?case by (auto intro: eff_S elim: epath.cases)
 qed
@@ -326,45 +325,45 @@ end \<comment> \<open>context RuleSystem\<close>
 
 (*<*) (* Rule-persistent rule system *) (*>*)
 locale PersistentRuleSystem = RuleSystem eff rules S
-for eff :: \<open>'rule \<Rightarrow> 'state \<Rightarrow> 'state fset \<Rightarrow> bool\<close> and rules :: \<open>'rule stream\<close> and S +
-assumes per: \<open>\<And> r. r \<in> R \<Longrightarrow> per r\<close>
+for eff :: "'rule \<Rightarrow> 'state \<Rightarrow> 'state fset \<Rightarrow> bool" and rules :: "'rule stream" and S +
+assumes per: "\<And> r. r \<in> R \<Longrightarrow> per r"
 begin
 
 lemma ipath_mkTree_saturated:
-  assumes s: \<open>s \<in> S\<close> and rs: \<open>fair rs\<close>
-  and i: \<open>ipath (mkTree rs s) steps\<close> and r: \<open>r \<in> R\<close>
-  shows \<open>saturated r steps\<close>
+  assumes s: "s \<in> S" and rs: "fair rs"
+  and i: "ipath (mkTree rs s) steps" and r: "r \<in> R"
+  shows "saturated r steps"
 unfolding saturated_def using s rs i proof (coinduction arbitrary: rs s steps)
   case (alw rs s steps)
   show ?case
   proof (intro exI[of _ steps], safe)
-    assume \<open>holds (enabledAtStep r) steps\<close>
-    hence \<open>alw (holds (enabledAtStep r)) steps \<or> ev (holds (takenAtStep r)) steps\<close>
+    assume "holds (enabledAtStep r) steps"
+    hence "alw (holds (enabledAtStep r)) steps \<or> ev (holds (takenAtStep r)) steps"
       by (rule variance[OF _ per_alw[OF per[OF r]]])
         (metis wf_ipath_epath wf_mkTree alw mkTree.simps(1) ipath.simps fst_conv)
-    thus \<open>ev (holds (takenAtStep r)) steps\<close> by (metis ipath_mkTree_ev[OF alw r])
+    thus "ev (holds (takenAtStep r)) steps" by (metis ipath_mkTree_ev[OF alw r])
   next
-    from alw show \<open>\<exists>rs' s' steps'.
-      stl steps = steps' \<and> s' \<in> S \<and> fair rs' \<and> ipath (mkTree rs' s') steps'\<close>
+    from alw show "\<exists>rs' s' steps'.
+      stl steps = steps' \<and> s' \<in> S \<and> fair rs' \<and> ipath (mkTree rs' s') steps'"
       using ipath_mkTree_sdrop[where m=1, simplified] trim_in_R sdrop_fair by fast
   qed
 qed
 
 theorem ipath_mkTree_Saturated:
-  assumes \<open>s \<in> S\<close> and \<open>fair rs\<close> and \<open>ipath (mkTree rs s) steps\<close>
-  shows \<open>Saturated steps\<close>
+  assumes "s \<in> S" and "fair rs" and "ipath (mkTree rs s) steps"
+  shows "Saturated steps"
   unfolding Saturated_def using ipath_mkTree_saturated[OF assms] by blast
 
 theorem epath_completeness_Saturated:
-  assumes \<open>s \<in> S\<close>
+  assumes "s \<in> S"
   shows
-  \<open>(\<exists> t. fst (root t) = s \<and> wf t \<and> tfinite t) \<or>
-   (\<exists> steps. fst (shd steps) = s \<and> epath steps \<and> Saturated steps)\<close> (is \<open>?A \<or> ?B\<close>)
+  "(\<exists> t. fst (root t) = s \<and> wf t \<and> tfinite t) \<or>
+   (\<exists> steps. fst (shd steps) = s \<and> epath steps \<and> Saturated steps)" (is "?A \<or> ?B")
 proof -
-  { assume \<open>\<not> ?A\<close>
-    with assms have \<open>\<not> tfinite (mkTree fenum s)\<close> using wf_mkTree fair_fenum by auto
-    then obtain steps where \<open>ipath (mkTree fenum s) steps\<close> using Konig by blast
-    with assms have \<open>fst (shd steps) = s \<and> epath steps \<and> Saturated steps\<close>
+  { assume "\<not> ?A"
+    with assms have "\<not> tfinite (mkTree fenum s)" using wf_mkTree fair_fenum by auto
+    then obtain steps where "ipath (mkTree fenum s) steps" using Konig by blast
+    with assms have "fst (shd steps) = s \<and> epath steps \<and> Saturated steps"
       by (metis wf_ipath_epath ipath.simps ipath_mkTree_Saturated
         wf_mkTree fair_fenum mkTree.simps(1) fst_conv)
     hence ?B by blast
@@ -382,26 +381,26 @@ section\<open>Code generation\<close>
 (* Here we assume a deterministic effect eff': *)
 
 locale RuleSystem_Code =
-fixes eff' :: \<open>'rule \<Rightarrow> 'state \<Rightarrow> 'state fset option\<close>
-and rules :: \<open>'rule stream\<close> \<comment> \<open>countably many rules\<close>
+fixes eff' :: "'rule \<Rightarrow> 'state \<Rightarrow> 'state fset option"
+and rules :: "'rule stream" \<comment> \<open>countably many rules\<close>
 begin
 
-definition \<open>eff r s sl \<equiv> eff' r s = Some sl\<close>
+definition "eff r s sl \<equiv> eff' r s = Some sl"
 
 end (* context RuleSystem_Code *)
 
-definition [code del]: \<open>effG eff' r s sl \<equiv> RuleSystem_Code.eff eff' r s sl\<close>
+definition [code del]: "effG eff' r s sl \<equiv> RuleSystem_Code.eff eff' r s sl"
 
 sublocale RuleSystem_Code < RuleSystem_Defs
-  where eff = \<open>effG eff'\<close> and rules = rules .
+  where eff = "effG eff'" and rules = rules .
 
 context RuleSystem_Code
 begin
 
-lemma enabled_eff': \<open>enabled r s \<longleftrightarrow> eff' r s \<noteq> None\<close>
+lemma enabled_eff': "enabled r s \<longleftrightarrow> eff' r s \<noteq> None"
 unfolding enabled_def effG_def eff_def by auto
 
-lemma pickEff_the[code]: \<open>pickEff r s = the (eff' r s)\<close>
+lemma pickEff_the[code]: "pickEff r s = the (eff' r s)"
 unfolding pickEff_def enabled_def effG_def eff_def by auto
 
 lemmas [code_unfold] = trim_def enabled_eff' pickEff_the
@@ -412,18 +411,18 @@ end (* context RuleSystem_Code *)
 
 setup Locale_Code.open_block
 interpretation i: RuleSystem_Code eff' rules for eff' and rules .
-declare [[lc_delete \<open>RuleSystem_Defs.mkTree (effG ?eff')\<close>]]
+declare [[lc_delete "RuleSystem_Defs.mkTree (effG ?eff')"]]
 declare [[lc_delete RuleSystem_Defs.trim]]
 declare [[lc_delete RuleSystem_Defs.enabled]]
 declare [[lc_delete RuleSystem_Defs.pickEff]]
-declare [[lc_add \<open>RuleSystem_Defs.mkTree (effG ?eff')\<close> i.mkTree_unfold]]
+declare [[lc_add "RuleSystem_Defs.mkTree (effG ?eff')" i.mkTree_unfold]]
 setup Locale_Code.close_block
 
 code_printing
   constant the \<rightharpoonup> (Haskell) "fromJust"
 | constant Option.is_none \<rightharpoonup> (Haskell) "isNothing"
 
-export_code mkTree_effG_uu in Haskell module_name Tree (*file \<open>.\<close>*)
+export_code mkTree_effG_uu in Haskell module_name Tree (*file "."*)
 
 (*<*)
 end
