thys/Completeness/Completeness.thy
@@ -890,6 +890,7 @@ lemma path_evalF':
 
 lemmas path_evalF'' = mp[OF path_evalF']
 
+
 subsection "adequacy"
 
 lemma counterAssignModelAssign: "counterAssign : modelAssigns (counterModel gamma)"
